TransVal/OutVars.v
@@ -1,0 +1,20 @@
+Require Import List.
+Require Import IL Val sexp.
+
+(** Inductive Predicate that is true if and only if the given list is a list of the output expressions of the
+IL/F program 
+The output expressions of a return statement is the list containing the expression that is returned.
+The output expressions of a function call is the list containing the expression in the call. **)
+Inductive OutVars: list exp -> stmt -> Prop :=
+| OutVarsRet e:  OutVars (e::nil) (stmtReturn e)
+| OutVarsFCall f e: OutVars e (stmtGoto f e)
+|OutVarsLet l x e s: OutVars l s -> OutVars l (stmtExp x e s)
+|OutVarsIf l1 l2 c t f : OutVars l1 t -> OutVars l2 f -> OutVars (List.app l1 l2) (stmtIf c t f)
+|OutVarsFun l Z s t: OutVars l  s -> OutVars l (stmtLet Z s t)
+|OutVarsExtern l x f Y s: OutVars l s -> OutVars l (stmtExtern x f Y s).
+
+(*
+*** Local Variables: ***
+*** coq-load-path: (("../" "Lvc")) ***
+*** End: ***
+*)
